src/library/constants.cpp
@@ -339,11 +339,24 @@ name const * g_sum_inl = nullptr;
 name const * g_sum_inr = nullptr;
 name const * g_tactic = nullptr;
 name const * g_tactic_constructor = nullptr;
-name const * g_tactic_interactive = nullptr;
 name const * g_tactic_step = nullptr;
 name const * g_tactic_to_expr = nullptr;
 name const * g_tactic_skip = nullptr;
 name const * g_tactic_try = nullptr;
+name const * g_tactic_interactive = nullptr;
+name const * g_tactic_interactive_types_ident = nullptr;
+name const * g_tactic_interactive_types_opt_ident = nullptr;
+name const * g_tactic_interactive_types_using_ident = nullptr;
+name const * g_tactic_interactive_types_ident_list = nullptr;
+name const * g_tactic_interactive_types_raw_ident_list = nullptr;
+name const * g_tactic_interactive_types_with_ident_list = nullptr;
+name const * g_tactic_interactive_types_location = nullptr;
+name const * g_tactic_interactive_types_comma_tk = nullptr;
+name const * g_tactic_interactive_types_qexpr = nullptr;
+name const * g_tactic_interactive_types_qexpr0 = nullptr;
+name const * g_tactic_interactive_types_qexpr_list = nullptr;
+name const * g_tactic_interactive_types_qexpr_list_or_qexpr0 = nullptr;
+name const * g_tactic_interactive_types_itactic = nullptr;
 name const * g_to_string = nullptr;
 name const * g_to_int = nullptr;
 name const * g_to_real = nullptr;
@@ -703,11 +716,24 @@ void initialize_constants() {
     g_sum_inr = new name{"sum", "inr"};
     g_tactic = new name{"tactic"};
     g_tactic_constructor = new name{"tactic", "constructor"};
-    g_tactic_interactive = new name{"tactic", "interactive"};
     g_tactic_step = new name{"tactic", "step"};
     g_tactic_to_expr = new name{"tactic", "to_expr"};
     g_tactic_skip = new name{"tactic", "skip"};
     g_tactic_try = new name{"tactic", "try"};
+    g_tactic_interactive = new name{"tactic", "interactive"};
+    g_tactic_interactive_types_ident = new name{"tactic", "interactive", "types", "ident"};
+    g_tactic_interactive_types_opt_ident = new name{"tactic", "interactive", "types", "opt_ident"};
+    g_tactic_interactive_types_using_ident = new name{"tactic", "interactive", "types", "using_ident"};
+    g_tactic_interactive_types_ident_list = new name{"tactic", "interactive", "types", "ident_list"};
+    g_tactic_interactive_types_raw_ident_list = new name{"tactic", "interactive", "types", "raw_ident_list"};
+    g_tactic_interactive_types_with_ident_list = new name{"tactic", "interactive", "types", "with_ident_list"};
+    g_tactic_interactive_types_location = new name{"tactic", "interactive", "types", "location"};
+    g_tactic_interactive_types_comma_tk = new name{"tactic", "interactive", "types", "comma_tk"};
+    g_tactic_interactive_types_qexpr = new name{"tactic", "interactive", "types", "qexpr"};
+    g_tactic_interactive_types_qexpr0 = new name{"tactic", "interactive", "types", "qexpr0"};
+    g_tactic_interactive_types_qexpr_list = new name{"tactic", "interactive", "types", "qexpr_list"};
+    g_tactic_interactive_types_qexpr_list_or_qexpr0 = new name{"tactic", "interactive", "types", "qexpr_list_or_qexpr0"};
+    g_tactic_interactive_types_itactic = new name{"tactic", "interactive", "types", "itactic"};
     g_to_string = new name{"to_string"};
     g_to_int = new name{"to_int"};
     g_to_real = new name{"to_real"};
@@ -1068,11 +1094,24 @@ void finalize_constants() {
     delete g_sum_inr;
     delete g_tactic;
     delete g_tactic_constructor;
-    delete g_tactic_interactive;
     delete g_tactic_step;
     delete g_tactic_to_expr;
     delete g_tactic_skip;
     delete g_tactic_try;
+    delete g_tactic_interactive;
+    delete g_tactic_interactive_types_ident;
+    delete g_tactic_interactive_types_opt_ident;
+    delete g_tactic_interactive_types_using_ident;
+    delete g_tactic_interactive_types_ident_list;
+    delete g_tactic_interactive_types_raw_ident_list;
+    delete g_tactic_interactive_types_with_ident_list;
+    delete g_tactic_interactive_types_location;
+    delete g_tactic_interactive_types_comma_tk;
+    delete g_tactic_interactive_types_qexpr;
+    delete g_tactic_interactive_types_qexpr0;
+    delete g_tactic_interactive_types_qexpr_list;
+    delete g_tactic_interactive_types_qexpr_list_or_qexpr0;
+    delete g_tactic_interactive_types_itactic;
     delete g_to_string;
     delete g_to_int;
     delete g_to_real;
@@ -1432,11 +1471,24 @@ name const & get_sum_inl_name() { return *g_sum_inl; }
 name const & get_sum_inr_name() { return *g_sum_inr; }
 name const & get_tactic_name() { return *g_tactic; }
 name const & get_tactic_constructor_name() { return *g_tactic_constructor; }
-name const & get_tactic_interactive_name() { return *g_tactic_interactive; }
 name const & get_tactic_step_name() { return *g_tactic_step; }
 name const & get_tactic_to_expr_name() { return *g_tactic_to_expr; }
 name const & get_tactic_skip_name() { return *g_tactic_skip; }
 name const & get_tactic_try_name() { return *g_tactic_try; }
+name const & get_tactic_interactive_name() { return *g_tactic_interactive; }
+name const & get_tactic_interactive_types_ident_name() { return *g_tactic_interactive_types_ident; }
+name const & get_tactic_interactive_types_opt_ident_name() { return *g_tactic_interactive_types_opt_ident; }
+name const & get_tactic_interactive_types_using_ident_name() { return *g_tactic_interactive_types_using_ident; }
+name const & get_tactic_interactive_types_ident_list_name() { return *g_tactic_interactive_types_ident_list; }
+name const & get_tactic_interactive_types_raw_ident_list_name() { return *g_tactic_interactive_types_raw_ident_list; }
+name const & get_tactic_interactive_types_with_ident_list_name() { return *g_tactic_interactive_types_with_ident_list; }
+name const & get_tactic_interactive_types_location_name() { return *g_tactic_interactive_types_location; }
+name const & get_tactic_interactive_types_comma_tk_name() { return *g_tactic_interactive_types_comma_tk; }
+name const & get_tactic_interactive_types_qexpr_name() { return *g_tactic_interactive_types_qexpr; }
+name const & get_tactic_interactive_types_qexpr0_name() { return *g_tactic_interactive_types_qexpr0; }
+name const & get_tactic_interactive_types_qexpr_list_name() { return *g_tactic_interactive_types_qexpr_list; }
+name const & get_tactic_interactive_types_qexpr_list_or_qexpr0_name() { return *g_tactic_interactive_types_qexpr_list_or_qexpr0; }
+name const & get_tactic_interactive_types_itactic_name() { return *g_tactic_interactive_types_itactic; }
 name const & get_to_string_name() { return *g_to_string; }
 name const & get_to_int_name() { return *g_to_int; }
 name const & get_to_real_name() { return *g_to_real; }
