library/init/meta/interactive.lean
@@ -4,26 +4,172 @@ Released under Apache 2.0 license as described in the file LICENSE.
 Authors: Leonardo de Moura
 -/
 prelude
-import init.meta.tactic
+import init.meta.tactic init.meta.rewrite_tactic
 
 namespace tactic
 namespace interactive
+namespace types
+/- The parser treats constants in the tactic.interactice namespace specially.
+   The following argument types have special parser support when interactive tactics
+   are used inside `begin ... end` blocks.
 
-meta def intro (h : name) : tactic unit :=
-tactic.intro h >> skip
+   - ident : make sure the next token is an identifier, and
+             produce the quoted name `t, where t is the next identifier.
 
-meta def apply (q : pexpr) : tactic unit :=
+   - opt_ident : parse (identifier)?
+
+   - using_ident
+
+   - raw_ident_list : parse identifier* and produce a list of quoted identifiers.
+
+         Example:
+           a b c
+         produces
+           [`a, `b, `c]
+
+   - with_ident_list : parse
+                 (`with` identifier+)?
+                 and produce a list of quoted identifiers
+   - comma_tk : parse the token `,` and produce the unit ()
+
+   - location : parse
+             (`at` identifier+)?
+             and produce a list of quoted identifiers
+
+   - qexpr : parse an expression e and produce the quoted expression `e
+
+   - qexpr_list : parse
+           `[` (expr (`,` expr)*)? `]`
+
+            and produce a list of quoted expressions.
+
+   - qexpr0 : parse an expression e using 0 as the right-binding-power,
+              and produce the quoted expression `e
+
+   - qexpr_list_or_qexpr0 : parse
+           `[` (expr (`,` expr)*)? `]`
+            or
+            expr
+
+            and produce a list of quoted expressions
+
+  - itactic: parse a nested "interactive" tactic -/
+def ident : Type := name
+def opt_ident : Type := option ident
+def using_ident : Type := option ident
+def raw_ident_list : Type := list ident
+def with_ident_list : Type := list ident
+def location : Type := list ident
+@[reducible] meta def qexpr : Type := pexpr
+@[reducible] meta def qexpr0 : Type := pexpr
+meta def qexpr_list : Type := list qexpr
+meta def qexpr_list_or_qexpr0 : Type := list qexpr
+meta def itactic : Type := tactic unit
+end types
+
+open types expr
+
+meta def intro : opt_ident → tactic unit
+| none     := intro1 >> skip
+| (some h) := tactic.intro h >> skip
+
+meta def intros : raw_ident_list → tactic unit
+| [] := tactic.intros >> skip
+| hs := intro_lst hs >> skip
+
+meta def apply (q : qexpr0) : tactic unit :=
 to_expr q >>= tactic.apply
 
-meta def refine : pexpr → tactic unit :=
+meta def refine : qexpr0 → tactic unit :=
 tactic.refine
 
 meta def assumption : tactic unit :=
 tactic.assumption
 
-meta def exact (e : pexpr) : tactic unit :=
+meta def change (q : qexpr0) : tactic unit :=
+to_expr_strict q >>= tactic.change
+
+meta def exact (q : qexpr0) : tactic unit :=
 do tgt : expr ← target,
-   to_expr_strict `((%%e : %%tgt)) >>= exact
+   to_expr_strict `((%%q : %%tgt)) >>= tactic.exact
+
+private meta def get_locals : list name → tactic (list expr)
+| []      := return []
+| (n::ns) := do h ← get_local n, hs ← get_locals ns, return (h::hs)
+
+meta def revert (ids : raw_ident_list) : tactic unit :=
+do hs ← get_locals ids, revert_lst hs, skip
+
+/- Return (some a) iff p is of the form (- a) -/
+private meta def is_neg (p : pexpr) : option pexpr :=
+/- Remark: we use the low-level to_raw_expr and of_raw_expr to be able to
+   pattern match pre-terms. This is a low-level trick (aka hack). -/
+match pexpr.to_raw_expr p with
+| (app (const c []) arg) := if c = `neg then some (pexpr.of_raw_expr arg) else none
+| _                      := none
+end
+
+private meta def to_symm_expr_list : list pexpr → tactic (list (bool × expr))
+| []      := return []
+| (p::ps) :=
+  match is_neg p with
+  | some a :=  do r ← to_expr a, rs ← to_symm_expr_list ps, return ((tt, r) :: rs)
+  | none   :=  do r ← to_expr p, rs ← to_symm_expr_list ps, return ((ff, r) :: rs)
+  end
+
+private meta def rw_goal : list (bool × expr) → tactic unit
+| []              := return ()
+| ((symm, e)::es) := rewrite_core reducible tt occurrences.all symm e >> rw_goal es
+
+private meta def rw_hyp : list (bool × expr) → name → tactic unit
+| []              hname := return ()
+| ((symm, e)::es) hname :=
+  do h ← get_local hname,
+     rewrite_at_core reducible tt occurrences.all symm e h,
+     rw_hyp es hname
+
+private meta def rw_hyps : list (bool × expr) → list name → tactic unit
+| es  []      := return ()
+| es  (h::hs) := rw_hyp es h >> rw_hyps es hs
+
+meta def rewrite (hs : qexpr_list_or_qexpr0) (loc : location) : tactic unit :=
+do hlist ← to_symm_expr_list hs,
+   match loc with
+   | [] := rw_goal hlist >> try reflexivity
+   | hs := rw_hyps hlist hs >> try reflexivity
+   end
+
+meta def rw : qexpr_list_or_qexpr0 → location → tactic unit :=
+rewrite
+
+private meta def get_type_name (e : expr) : tactic name :=
+do e_type ← infer_type e >>= whnf,
+   (const I ls) ← return $ get_app_fn e_type | failed,
+   return I
+
+meta def induction (p : qexpr0) (rec_name : using_ident) (ids : with_ident_list) : tactic unit :=
+do e ← to_expr p,
+   match rec_name with
+   | some n := induction_core semireducible e n ids
+   | none   := do I ← get_type_name e, induction_core semireducible e (I <.> "rec") ids
+   end
+
+meta def cases (p : qexpr0) (ids : with_ident_list) : tactic unit :=
+do e ← to_expr p,
+   cases_core semireducible e ids
+
+meta def generalize (p : qexpr) (x : ident) : tactic unit :=
+do e ← to_expr p,
+   tactic.generalize e x
+
+meta def trivial : tactic unit :=
+tactic.triv <|> tactic.reflexivity <|> tactic.contradiction
+
+meta def contradiction : tactic unit :=
+tactic.contradiction
+
+meta def repeat : itactic → tactic unit :=
+tactic.repeat
 
 end interactive
 end tactic
