library/init/meta/pexpr.lean
@@ -9,8 +9,12 @@ universe variables u
 
 /- Quoted expressions. They can be converted into expressions by using a tactic. -/
 meta constant pexpr : Type
-protected meta constant pexpr.of_expr : expr → pexpr
-protected meta constant pexpr.subst   : pexpr → pexpr → pexpr
+protected meta constant pexpr.of_expr  : expr → pexpr
+protected meta constant pexpr.subst    : pexpr → pexpr → pexpr
+
+/- Low level primitives for accessing internal representation. -/
+protected meta constant pexpr.to_raw_expr : pexpr → expr
+protected meta constant pexpr.of_raw_expr : expr → pexpr
 
 meta constant pexpr.to_string : pexpr → string
 meta instance : has_to_string pexpr :=
