tests/lean/run/auto_quote1.lean
@@ -1,6 +1,6 @@
 example (a b c : nat) : a = b → b = c → c = a :=
 begin
-  tactic.intros,
+  intros,
   apply eq.symm,
   apply eq.trans,
   assumption,
@@ -13,4 +13,50 @@ begin
   intro h2,
   refine eq.symm (eq.trans h1 _),
   exact h2
+end
+
+example (a b c : nat) : a = b → b = c → c = a :=
+begin
+  intros h1 h2, -- we can optionally provide the names
+  refine eq.symm (eq.trans h1 _),
+  exact h2
+end
+
+example (a b c : nat) : a = b → b = c → c = a :=
+begin
+  intro h1,
+  intro, -- optional argument
+  refine eq.symm (eq.trans h1 _),
+  assumption
+end
+
+constant add_comm {a b : nat} : a + b = b + a
+constant add_assoc {a b c : nat} : (a + b) + c = a + (b + c)
+constant zero_add (a : nat) : 0 + a = a
+
+example (a b c : nat) : b = 0 → 0 + a + b + c = c + a :=
+begin
+  intro h,
+  rewrite h, -- single rewrite
+  rewrite [zero_add, @add_comm a 0, zero_add, add_comm] -- sequence of rewrites
+end
+
+example (a b c : nat) : 0 = b → 0 + a + b + c = c + a :=
+begin
+  intro h,
+  rewrite -h, -- single rewrite using symmetry
+  rw [zero_add, @add_comm a 0, zero_add, add_comm] -- rw is shorthand for rewrite
+end
+
+open nat
+
+example : ∀ n m : ℕ, n + m = m + n :=
+begin
+  intros n m,
+  induction m with m' ih,
+  { -- Remark: Used change here to make sure nat.zero is replaced with polymorphic zero.
+    -- dsimp tactic should fix that in the future.
+    change n + 0 = 0 + n, rw zero_add n },
+  { change succ (n + m') = succ m' + n,
+    rw [succ_add, ih] }
 end
